added popStackFrame and another example

examples/low-level/example1.fst
@@ -12,22 +12,25 @@ open Prims
 open List
 open ListSet
 
-val helloWorld : unit -> SST unit  (fun m -> True) (fun m0 a m1 -> True)
-let helloWorld () = (newStackFrame ())
-
-
 
 (*a good aspect of the current formulation is that the heap/stack difference
 only matters at the time of allocation. Functions like increment can be
 defined without without bothering about that distinction*)
-val increment : r:(ref int) -> SST unit  (fun m -> (refExistsInMem r m)==true) (fun m0 a m1 -> True)
-let increment r =
+
+(*ideally, the refExistsInMem clauses should not be needed in the postcondition*)
+val incrementRef : r:(ref int) -> SST unit  (fun m -> (refExistsInMem r m)==true)
+(fun m0 a m1 -> (refExistsInMem r m0) /\ (refExistsInMem r m1) /\ (loopkupRef r m1 = (loopkupRef r m0) + 1))
+let incrementRef r =
   let oldv = read r in
   write r (oldv + 1)
 
-(*ideally, the refExistsInMem clauses should not be needed in the postcondition*)
-val increment2 : r:(ref int) -> SST unit  (fun m -> (refExistsInMem r m)==true)
-(fun m0 a m1 -> (refExistsInMem r m0) /\ (refExistsInMem r m1) /\ (loopkupRef r m1 = (loopkupRef r m0) + 1))
-let increment2 r =
-  let oldv = read r in
-  write r (oldv + 1)
+val incrementUsingStack : vi:int -> SST int  (fun _ -> True) (fun m0 vo m1 -> m0=m1 /\ vo=vi+1)
+
+val incrementUsingStack : vi:int -> SST int  (fun _ -> True) (fun m0 vo m1 -> True)
+let incrementUsingStack vi =
+  pushStackFrame ();
+    let r = salloc vi in
+    incrementRef r;
+    let v = (read r) in
+  popStackFrame ();
+  v
